src/PairHeap.fst
@@ -191,6 +191,11 @@ val mem_insert : h:intHeap -> i:int ->
         (ensures (forall j. mem j (insert h i) <==> j = i \/ mem j h))
 let mem_insert h i = mem_merge h (Heap (i, []))
 
+val elts_insert : h:intHeap -> i:int ->
+  Lemma (requires true)
+	(ensures  (elts (insert h i) = ins i (elts h)))
+let elts_insert h i = ()
+
 (* Correctness properties *)
 val leq_is_min : i:int -> h:intHeap{is_heap h} ->
   Lemma (requires (leq_heap i h))
